Update Sequent.thy

Sequent.thy
@@ -12,13 +12,11 @@ text \<open>
 \<close>
 datatype ('f) tm  = Var nat | Fun 'f \<open>nat list\<close>
 
-
+datatype sign = pos | neg
 datatype ('f) form = 
-    EqAtom "'f tm" "'f tm"
-  | NEqAtom "'f tm" "'f tm"
+    EqAtom sign "'f tm" "'f tm"
   | ConcEq "'f tm" "'f tm" "'f tm"
-  | Member "'f tm" "char BA rexp"
-  | NMember "'f tm" "char BA rexp"
+  | Member sign "'f tm" "char BA rexp"
   | Dis "'f form" "'f form"                     
   | Con "'f form" "'f form"                      
   | Neg "'f form"     
@@ -32,16 +30,17 @@ primrec params_tm :: "'f tm \<Rightarrow> nat set" where
   "params_tm (Fun f ns) = set ns"
 
 primrec params_fm :: "'f form \<Rightarrow> nat set" where
-  "params_fm (EqAtom f1 f2) = (params_tm f1 \<union> params_tm f2)"|
-  "params_fm (NEqAtom f1 f2) = (params_tm f1 \<union> params_tm f2)"|
+  "params_fm (EqAtom s f1 f2) = (params_tm f1 \<union> params_tm f2)"|
   "params_fm (ConcEq f1 f2 f3) = (params_tm f1 \<union> params_tm f2 \<union> params_tm f3)"|
-  "params_fm (Member f r) = (params_tm f)"|
-  "params_fm (NMember f r) = (params_tm f)"|
+  "params_fm (Member s f r) = (params_tm f)"|
   "params_fm (Dis f1 f2) = (params_fm f1 \<union> params_fm f2)"|
   "params_fm (Con f1 f2) = (params_fm f1 \<union> params_fm f2)"|
   "params_fm (Neg f) = (params_fm f)"|
   "params_fm (FF) = {}"|
   "params_fm TT = {}"
+
+definition fresh :: "'f tm \<Rightarrow> 'f tm \<Rightarrow> nat list \<Rightarrow> bool" where 
+"fresh x y xs = (\<not> params_tm y \<subseteq> (params_tm x \<union> set xs))"
 
 abbreviation \<open>params S \<equiv> \<Union>p \<in> S. params_fm p\<close>
 
@@ -55,11 +54,9 @@ fun concat_str :: "string \<Rightarrow> string list \<Rightarrow> string" where
 "concat_str s ls = (if s = ''concat'' then List.concat ls else [])"
 
 primrec semantics_fm (\<open>\<lbrakk>_, _\<rbrakk>\<close>) where
-  \<open>\<lbrakk>E, F\<rbrakk> (EqAtom x y) = (\<lparr>E, F\<rparr> x = \<lparr>E, F\<rparr> y)\<close> 
-| \<open>\<lbrakk>E, F\<rbrakk> (NEqAtom x y) = (\<lparr>E, F\<rparr> x \<noteq> \<lparr>E, F\<rparr> y)\<close> 
+  \<open>\<lbrakk>E, F\<rbrakk> (EqAtom s x y) = (if s = pos then \<lparr>E, F\<rparr> x = \<lparr>E, F\<rparr> y else \<lparr>E, F\<rparr> x \<noteq> \<lparr>E, F\<rparr> y)\<close> 
 | \<open>\<lbrakk>E, F\<rbrakk> (ConcEq z x y) = (\<lparr>E, F\<rparr> z = \<lparr>E, F\<rparr> x @ \<lparr>E, F\<rparr> y)\<close> 
-| \<open>\<lbrakk>E, F\<rbrakk> (Member x r) = (\<lparr>E, F\<rparr> x \<in> lang r)\<close> 
-| \<open>\<lbrakk>E, F\<rbrakk> (NMember x r) = (\<lparr>E, F\<rparr> x \<notin> lang r)\<close> 
+| \<open>\<lbrakk>E, F\<rbrakk> (Member s x r) = (if s = pos then \<lparr>E, F\<rparr> x \<in> lang r else \<lparr>E, F\<rparr> x \<notin> lang r)\<close> 
 | \<open>\<lbrakk>E, F\<rbrakk> (Dis x y) = (\<lbrakk>E, F\<rbrakk> x \<or> \<lbrakk>E, F\<rbrakk> y)\<close> 
 | \<open>\<lbrakk>E, F\<rbrakk> (Con x y) = (\<lbrakk>E, F\<rbrakk> x \<and> \<lbrakk>E, F\<rbrakk> y)\<close> 
 | \<open>\<lbrakk>E, F\<rbrakk> (Neg x) = (\<not> \<lbrakk>E, F\<rbrakk> x)\<close> 
@@ -69,15 +66,15 @@ primrec semantics_fm (\<open>\<lbrakk>_, _\<rbrakk>\<close>) where
 subsection \<open>Proof System\<close>
 
 fun is_Member :: "'f form \<Rightarrow> bool" where 
-  "is_Member (Member x r)  = True"|
+  "is_Member (Member s x r)  = True"|
   "is_Member _ = False"
 
 fun variable_in_member :: "'f form \<Rightarrow> 'f tm option" where 
-"variable_in_member (Member x r) = Some x"|
+"variable_in_member (Member s x r) = Some x"|
 "variable_in_member _ = None"
 
 fun rexp_in_member :: "'f form \<Rightarrow> char BA rexp  " where 
-"rexp_in_member (Member x r) = r"
+"rexp_in_member (Member s x r) = r"
 
 definition "distinct_variable  ls = distinct (map (variable_in_member) ls)"
 
@@ -102,7 +99,7 @@ fun eq_len_intersect :: "char BA rexp \<Rightarrow> char BA rexp list \<Rightarr
 fun member_var_rexp :: "nat list \<Rightarrow> char BA rexp list \<Rightarrow> string form list" where 
 "member_var_rexp [] b = []"|
 "member_var_rexp (v # va) [] = []"|
-"member_var_rexp (x#xs) (y#ys) = (if (length xs = length ys) then (Member (Var x) y) # (member_var_rexp xs ys) else [])"
+"member_var_rexp (x#xs) (y#ys) = (if (length xs = length ys) then (Member pos (Var x) y) # (member_var_rexp xs ys) else [])"
 
 fun con_fwd_prop ::"char BA rexp \<Rightarrow> char BA rexp \<Rightarrow> char BA rexp \<Rightarrow> bool" where
 "con_fwd_prop r e1 r2 = (lang (r) = lang (Times e1 r2))"
@@ -119,21 +116,21 @@ inductive One_SC :: \<open>string form list  \<Rightarrow> bool\<close> (\<open>
 | AlphaOr:       \<open>\<stileturn> A# \<Gamma> \<Longrightarrow> \<stileturn> B# \<Gamma> \<Longrightarrow> \<stileturn> Dis A B # \<Gamma>\<close>
 | AlphaNegAnd:   \<open>\<stileturn> Neg A # \<Gamma> \<Longrightarrow>  \<stileturn> Neg B # \<Gamma> \<Longrightarrow> \<stileturn> Neg (Con A B) # \<Gamma>\<close>
 | AlphaNegNeg:   \<open>\<stileturn> A# \<Gamma> \<Longrightarrow> \<stileturn> Neg (Neg A) # \<Gamma>\<close>
-| NotMember:     \<open>regexp_compl e ec \<Longrightarrow> \<stileturn> (Member x ec) # \<Gamma> \<Longrightarrow> \<stileturn> (NMember x e) # \<Gamma>\<close>
-| NotEq:         \<open>\<stileturn> [NEqAtom x y,  EqAtom y (Fun f xs), \<Gamma>] \<Longrightarrow> \<stileturn> [NEqAtom x (Fun f xs), \<Gamma>]\<close>
-| Cut:           \<open>regexp_compl e ec \<Longrightarrow> \<stileturn> Member x e # \<Gamma> \<Longrightarrow>  \<stileturn> Member x ec # \<Gamma> \<Longrightarrow>  \<stileturn> \<Gamma>\<close>
-| EqProp:        \<open>\<stileturn> Member x e # EqAtom x y # Member y e # \<Gamma> \<Longrightarrow> \<stileturn> Member x e # EqAtom x y # \<Gamma>\<close>
-| NeqSubsume:    \<open>regexp_empty e1 e2 \<Longrightarrow> \<stileturn> Member x e1 # Member y e2 # \<Gamma> \<Longrightarrow> \<stileturn> Member x e1 # NEqAtom x y # Member y e2 # \<Gamma>\<close>
-| EqPropElim:    \<open>is_singleton (lang e) \<Longrightarrow> \<stileturn> Member x e # Member y e # \<Gamma>\<Longrightarrow> \<stileturn> Member x e # (EqAtom x y) # \<Gamma>\<close>
-| NeqPropElim:   \<open>is_singleton (lang e) \<Longrightarrow> regexp_compl e ec \<Longrightarrow> \<stileturn> (Member x e) # (Member y ec) # \<Gamma> \<Longrightarrow>  
-                 \<stileturn> (Member x e) # (NEqAtom x y) # \<Gamma>\<close>
-| Close:         \<open>empty_intersection_set rs \<Longrightarrow> \<stileturn> [FF] \<Longrightarrow> \<stileturn> map (\<lambda>r. Member x r) rs\<close> 
-| Subsume:       \<open>subset_intersect_set e fs \<Longrightarrow> \<stileturn> (map (\<lambda>r. Member x r) fs) @ \<Gamma> \<Longrightarrow> \<stileturn> Member x e # (map (\<lambda>r. Member x r) fs) @ \<Gamma>\<close> 
-| Intersect:     \<open>eq_len_intersect e fs \<Longrightarrow> \<stileturn> Member x e # \<Gamma>  \<Longrightarrow>  \<stileturn> (map (\<lambda>r. Member x r) (fs)) @ \<Gamma>\<close> 
-| Fwd_PropConc:  \<open>con_fwd_prop e e1 e2 \<Longrightarrow> \<stileturn> [(Member x e), (EqAtom x (Fun ''concat'' [x1,x2])), (Member (Var x1) e1), (Member (Var x2) e2)] @ \<Gamma>
-                 \<Longrightarrow> \<stileturn> [(EqAtom x (Fun ''concat'' [x1,x2])), (Member (Var x1) e1), (Member (Var x2) e2)] @ \<Gamma>\<close>  
-| Fwd_ElimConc:  \<open>con_fwd_prop_elim e e1 e2 \<Longrightarrow> \<stileturn> [Member x e, (Member (Var x1) e1), (Member (Var x2) e2)]  @ \<Gamma> \<Longrightarrow>  
-                 \<stileturn> [(EqAtom x (Fun ''concat'' [x1, x2])), (Member (Var x1) e1), (Member (Var x2) e2)] @ \<Gamma>\<close>
+| NotMember:     \<open>regexp_compl e ec \<Longrightarrow> \<stileturn> (Member pos x ec) # \<Gamma> \<Longrightarrow> \<stileturn> (Member neg x e) # \<Gamma>\<close>
+| NotEq:         \<open>\<stileturn> [EqAtom neg x y,  EqAtom pos y (Fun f xs), \<Gamma>] \<Longrightarrow> \<stileturn> [EqAtom neg x (Fun f xs), \<Gamma>]\<close>
+| Cut:           \<open>regexp_compl e ec \<Longrightarrow> \<stileturn> Member pos x e # \<Gamma> \<Longrightarrow>  \<stileturn> Member pos x ec # \<Gamma> \<Longrightarrow>  \<stileturn> \<Gamma>\<close>
+| EqProp:        \<open>\<stileturn> Member pos x e # EqAtom pos x y # Member pos y e # \<Gamma> \<Longrightarrow> \<stileturn> Member pos x e # EqAtom pos x y # \<Gamma>\<close>
+| NeqSubsume:    \<open>regexp_empty e1 e2 \<Longrightarrow> \<stileturn> Member pos x e1 # Member pos y e2 # \<Gamma> \<Longrightarrow> \<stileturn> Member pos x e1 # EqAtom neg x y # Member pos y e2 # \<Gamma>\<close>
+| EqPropElim:    \<open>is_singleton (lang e) \<Longrightarrow> \<stileturn> Member pos x e # Member pos y e # \<Gamma>\<Longrightarrow> \<stileturn> Member pos x e # (EqAtom pos x y) # \<Gamma>\<close>
+| NeqPropElim:   \<open>is_singleton (lang e) \<Longrightarrow> regexp_compl e ec \<Longrightarrow> \<stileturn> (Member pos x e) # (Member pos y ec) # \<Gamma> \<Longrightarrow>  
+                 \<stileturn> (Member pos x e) # (EqAtom neg x y) # \<Gamma>\<close>
+| Close:         \<open>empty_intersection_set rs \<Longrightarrow> \<stileturn> [FF] \<Longrightarrow> \<stileturn> map (\<lambda>r. Member pos x r) rs\<close> 
+| Subsume:       \<open>subset_intersect_set e fs \<Longrightarrow> \<stileturn> (map (\<lambda>r. Member pos x r) fs) @ \<Gamma> \<Longrightarrow> \<stileturn> Member pos x e # (map (\<lambda>r. Member pos x r) fs) @ \<Gamma>\<close> 
+| Intersect:     \<open>eq_len_intersect e fs \<Longrightarrow> \<stileturn> Member pos x e # \<Gamma>  \<Longrightarrow>  \<stileturn> (map (\<lambda>r. Member pos x r) (fs)) @ \<Gamma>\<close> 
+| Fwd_PropConc:  \<open>con_fwd_prop e e1 e2 \<Longrightarrow> \<stileturn> [(Member pos x e), (EqAtom pos x (Fun ''concat'' [x1,x2])), (Member pos (Var x1) e1), (Member pos (Var x2) e2)] @ \<Gamma>
+                 \<Longrightarrow> \<stileturn> [(EqAtom pos x (Fun ''concat'' [x1,x2])), (Member pos (Var x1) e1), (Member pos (Var x2) e2)] @ \<Gamma>\<close>  
+| Fwd_ElimConc:  \<open>con_fwd_prop_elim e e1 e2 \<Longrightarrow> \<stileturn> [Member pos x e, (Member pos (Var x1) e1), (Member pos (Var x2) e2)]  @ \<Gamma> \<Longrightarrow>  
+                 \<stileturn> [(EqAtom pos x (Fun ''concat'' [x1, x2])), (Member pos (Var x1) e1), (Member pos (Var x2) e2)] @ \<Gamma>\<close>
 (*| Bwd_PropConc:  \<open>con_bwd_prop e = es \<Longrightarrow> \<stileturn> ((\<lambda>r. [Member x e, EqAtom x (Fun ''concat'' [x1,x2]), Member (Var x1) (fst r), Member (Var x2) (snd r)] @ \<Gamma>) ` es) \<Longrightarrow> 
                  \<stileturn> {[Member x e, EqAtom x (Fun ''concat'' [x1,x2])] @ \<Gamma>}\<close>*)
 | Order:         \<open>\<stileturn> G \<Longrightarrow> set G = set G' \<Longrightarrow> \<stileturn> G'\<close>
@@ -141,14 +138,14 @@ inductive One_SC :: \<open>string form list  \<Rightarrow> bool\<close> (\<open>
 
 declare One_SC.intros [intro]
 
-(*lemma "\<stileturn> {((map (\<lambda>r. Member x r) [Pred (Atom CHR ''b''), Pred (Atom CHR ''a'')] @ []))}"
+(*lemma "\<stileturn> {((map (\<lambda>r. Member pos x r) [Pred (Atom CHR ''b''), Pred (Atom CHR ''a'')] @ []))}"
   apply (rule Close)
   subgoal apply auto done
   apply (rule Basic) 
   done
 
 
-lemma "\<stileturn> {((map (\<lambda>r. Member x r) [Pred (Atom CHR ''b''), Pred (Atom CHR ''a'')] @ []))}"
+lemma "\<stileturn> {((map (\<lambda>r. Member pos x r) [Pred (Atom CHR ''b''), Pred (Atom CHR ''a'')] @ []))}"
   apply (rule Close)
   apply (auto simp:distinct_variable_def single_word_def)
   done
@@ -170,11 +167,11 @@ next
     by (metis is_singletonE singletonD)
 next
   case (NeqPropElim e ec x y \<Gamma>)
-  then show ?case apply (auto simp: is_singleton_def) done 
+  then show ?case apply (auto simp: is_singleton_def)  done 
 next
   case (Subsume e fs x \<Gamma>)
   then show ?case apply auto 
-    by (smt (verit) INT_I Un_iff image_iff semantics_fm.simps(4) subsetD)  
+    by (smt (verit, ccfv_SIG) INT_I image_subset_iff semantics_fm.simps(3) subsetD sup.cobounded1)
 next
   case (Intersect e fs x \<Gamma>)
   then show ?case  apply auto 
@@ -211,26 +208,26 @@ following holds:
 
 definition consistency :: \<open>string form set set \<Rightarrow> bool\<close> where
   \<open>consistency C = (\<forall>S. S \<in> C \<longrightarrow> FF \<notin> S \<and> 
-               (\<forall>p q. \<not> (EqAtom p q \<in> S \<and> NEqAtom p q \<in> S) \<and>
-               \<not> (\<forall>x r. Member x r \<in> S \<and> NMember x r \<in> S)) \<and> 
+               (\<forall>p q. \<not> (EqAtom pos p q \<in> S \<and> EqAtom neg  p q \<in> S) \<and>
+               \<not> (\<forall>x r. Member pos x r \<in> S \<and> Member pos x r \<in> S)) \<and> 
               (\<forall> A B. Con A B \<in> S \<longrightarrow> S \<union> {A, B} \<in> C) \<and> 
               (\<forall> A B. Neg (Dis A B) \<in> S \<longrightarrow> S \<union> {Neg A, Neg B} \<in> C) \<and> 
               (\<forall> A B. Dis A B \<in> S \<longrightarrow> S \<union> {A} \<in> C \<or> S \<union> {B} \<in> C) \<and> 
               (\<forall> A B. Neg (Con A B) \<in> S \<longrightarrow> S \<union> {Neg A} \<in> C \<or> S \<union> {Neg B} \<in> C) \<and> 
               (\<forall> A. Neg (Neg A) \<in> S \<longrightarrow> S \<union> {A} \<in> C) \<and> 
-              (\<forall> x e ec. regexp_compl e ec \<longrightarrow> NMember x e \<in> S \<longrightarrow> S \<union> {Member x ec} \<in> C ) \<and> 
-              (\<forall> x y f xs. NEqAtom x (Fun f xs) \<in> S \<longrightarrow> S \<union> {NEqAtom x y, EqAtom y (Fun f xs)} \<in> C) \<and> 
-              (\<forall> x e ec. regexp_compl e ec \<longrightarrow> S \<union> {Member x e} \<in> C \<or> S \<union> {Member x ec} \<in> C) \<and> 
-              (\<forall> x y e. Member x e \<in> S \<and> EqAtom x y \<in> S \<longrightarrow> S \<union> {Member x e, EqAtom x y, Member y e} \<in> C) \<and> 
-              (\<forall> e1 e2 x y. regexp_empty e1 e2 \<longrightarrow> Member x e1 \<in> S \<and> NEqAtom x y \<in> S \<and> Member y e2 \<in> S \<longrightarrow> S \<union> {Member x e1, Member y e2} \<in> C) \<and>
-              (\<forall> x y e. is_singleton (lang e) \<longrightarrow> Member x e \<in> S \<and> EqAtom x y \<in> S \<longrightarrow> S \<union> {Member x e, Member y e} \<in> C) \<and> 
-              (\<forall> x y e ec. is_singleton (lang e) \<longrightarrow> regexp_compl e ec \<longrightarrow> Member x e \<in> S \<and> NEqAtom x y \<in> S \<longrightarrow> S \<union> {Member x e, Member y ec} \<in> C) \<and> 
-              (\<forall> x rs. empty_intersection_set rs \<longrightarrow> S \<union> ((\<lambda>r. Member x r) ` (set rs)) \<in> C \<longrightarrow> S \<union> {FF} \<in> C) \<and> 
-              (\<forall> x e fs. subset_intersect_set e fs \<longrightarrow> Member x e \<in> S \<and> S \<union> ((\<lambda>r. Member x r)) ` (set fs) \<in> C \<longrightarrow> S \<union> ((\<lambda>r. Member x r)) ` (set fs) \<in> C) \<and> 
-              (\<forall> x e fs. eq_len_intersect e fs \<longrightarrow>  S \<union> ((\<lambda>r. Member x r)) ` (set fs) \<in> C \<longrightarrow> S \<union> {Member x e} \<in> C) \<and> 
-              (\<forall> x x1 x2 e e1 e2 f. con_fwd_prop e e1 e2 \<longrightarrow> EqAtom x (Fun f [x1, x2]) \<in> S \<and> Member (Var x1) e1 \<in> S \<and> Member (Var x2) e2 \<in> S \<longrightarrow> S \<union> {Member x e, EqAtom x (Fun f [x1,x2]), Member (Var x1) e1, Member (Var x2) e2} \<in> C) \<and> 
-              (\<forall> x x1 x2 e e1 e2 f. con_fwd_prop_elim e e1 e2 \<longrightarrow> EqAtom x (Fun f [x1, x2]) \<in> S \<and> Member (Var x1) e1 \<in> S \<and> Member (Var x2) e2 \<in> S \<longrightarrow> S \<union> {Member x e, Member (Var x1) e1, Member (Var x2) e2} \<in> C) \<and> 
-              (\<forall> S'. S' = S \<longrightarrow> S' \<in> C)) \<close>
+              (\<forall> x e ec. regexp_compl e ec \<longrightarrow> Member neg x e \<in> S \<longrightarrow> S \<union> {Member pos x ec} \<in> C ) \<and> 
+              (\<forall> x y f xs. EqAtom neg  x (Fun f xs) \<in> S \<longrightarrow> S \<union> {EqAtom neg  x y, EqAtom pos y (Fun f xs)} \<in> C) \<and> 
+              (\<forall> x e ec. regexp_compl e ec \<longrightarrow> S \<union> {Member pos x e} \<in> C \<or> S \<union> {Member pos x ec} \<in> C) \<and> 
+              (\<forall> x y e. Member pos x e \<in> S \<and> EqAtom pos x y \<in> S \<longrightarrow> S \<union> {Member pos x e, EqAtom pos x y, Member pos y e} \<in> C) \<and> 
+              (\<forall> e1 e2 x y. regexp_empty e1 e2 \<longrightarrow> Member pos x e1 \<in> S \<and> EqAtom neg  x y \<in> S \<and> Member pos y e2 \<in> S \<longrightarrow> S \<union> {Member pos x e1, Member pos y e2} \<in> C) \<and>
+              (\<forall> x y e. is_singleton (lang e) \<longrightarrow> Member pos x e \<in> S \<and> EqAtom pos x y \<in> S \<longrightarrow> S \<union> {Member pos x e, Member pos y e} \<in> C) \<and> 
+              (\<forall> x y e ec. is_singleton (lang e) \<longrightarrow> regexp_compl e ec \<longrightarrow> Member pos x e \<in> S \<and> EqAtom neg  x y \<in> S \<longrightarrow> S \<union> {Member pos x e, Member pos y ec} \<in> C) \<and> 
+              (\<forall> x rs. empty_intersection_set rs \<longrightarrow> S \<union> ((\<lambda>r. Member pos x r) ` (set rs)) \<in> C \<longrightarrow> S \<union> {FF} \<in> C) \<and> 
+              (\<forall> x e fs. subset_intersect_set e fs \<longrightarrow> Member pos x e \<in> S \<and> S \<union> ((\<lambda>r. Member pos x r)) ` (set fs) \<in> C \<longrightarrow> S \<union> ((\<lambda>r. Member pos x r)) ` (set fs) \<in> C) \<and> 
+              (\<forall> x e fs. eq_len_intersect e fs \<longrightarrow>  S \<union> ((\<lambda>r. Member pos x r)) ` (set fs) \<in> C \<longrightarrow> S \<union> {Member pos x e} \<in> C) \<and> 
+              (\<forall> x x1 x2 e e1 e2 f. con_fwd_prop e e1 e2 \<longrightarrow> EqAtom pos x (Fun f [x1, x2]) \<in> S \<and> Member pos (Var x1) e1 \<in> S \<and> Member pos (Var x2) e2 \<in> S \<longrightarrow> S \<union> {Member pos x e, EqAtom pos x (Fun f [x1,x2]), Member pos (Var x1) e1, Member pos (Var x2) e2} \<in> C) \<and> 
+              (\<forall> x x1 x2 e e1 e2 f. con_fwd_prop_elim e e1 e2 \<longrightarrow> EqAtom pos x (Fun f [x1, x2]) \<in> S \<and> Member pos (Var x1) e1 \<in> S \<and> Member pos (Var x2) e2 \<in> S \<longrightarrow> S \<union> {Member pos x e, Member pos (Var x1) e1, Member pos (Var x2) e2} \<in> C) \<and> 
+              (\<forall> S'. S' = S \<longrightarrow> S' \<in> C))\<close>
 
 subsection \<open>Completeness\<close>
 
